theories/heap_lang/lib/spawn.v
@@ -20,7 +20,7 @@ Definition join : val :=
 (** The CMRA & functor we need. *)
 (* Not bundling heapG, as it may be shared with other users. *)
 Class spawnG Σ := SpawnG { spawn_tokG :> inG Σ (exclR unitC) }.
-Definition spawnΣ : gFunctors := #[GFunctor (constRF (exclR unitC))].
+Definition spawnΣ : gFunctors := #[GFunctor (exclR unitC)].
 
 Instance subG_spawnΣ {Σ} : subG spawnΣ Σ → spawnG Σ.
 Proof. intros [?%subG_inG _]%subG_inv. split; apply _. Qed.
