theories/heap_lang/lib/spin_lock.v
@@ -15,7 +15,7 @@ Definition release : val := λ: "l", "l" <- #false.
 (** The CMRA we need. *)
 (* Not bundling heapG, as it may be shared with other users. *)
 Class lockG Σ := LockG { lock_tokG :> inG Σ (exclR unitC) }.
-Definition lockΣ : gFunctors := #[GFunctor (constRF (exclR unitC))].
+Definition lockΣ : gFunctors := #[GFunctor (exclR unitC)].
 
 Instance subG_lockΣ {Σ} : subG lockΣ Σ → lockG Σ.
 Proof. intros ?%subG_inG. split; apply _. Qed.
