theories/tests/counter.v
@@ -73,7 +73,7 @@ Section M.
 End M.
 
 Class counterG Σ := CounterG { counter_tokG :> inG Σ M_UR }.
-Definition counterΣ : gFunctors := #[GFunctor (constRF M_UR)].
+Definition counterΣ : gFunctors := #[GFunctor M_UR].
 Instance subG_counterΣ {Σ} : subG counterΣ Σ → counterG Σ.
 Proof. intros [?%subG_inG _]%subG_inv. split; apply _. Qed.
 
